Hmm... should we be tagging variables with a kind...

LogicalRefinement/Stlc/InterpIrrel.lean
@@ -1,7 +1,31 @@
 import LogicalRefinement.Untyped
 import LogicalRefinement.Typed
 import LogicalRefinement.Stlc.Basic
+import LogicalRefinement.Stlc.Interp
 import LogicalRefinement.Stlc.Irrel
 import LogicalRefinement.Utils
 open Annot
 open AnnotSort
+
+def Context.is_irrel (Γ: Context) (n: Nat): Prop
+  := ∃A, ∃k, k ≠ HypKind.val type ∧ HasVar Γ n k A
+
+def Context.is_rel (Γ: Context) (n: Nat): Prop
+  := ∃A, HasVar Γ n (HypKind.val type) A
+
+@[simp] def Stlc.Context.interp.eq_mod_lrt 
+  {Γ: Stlc.Context} (G G': Γ.interp) (Γ: _root_.Context): Prop
+  := ∀n: Nat, Γ.is_rel n -> eq_at G G' n
+
+theorem HasType.interp_irrel_dep {Γ a A} (H: Γ ⊢ a: expr type A) (n: Nat):
+  a.stlc.has_dep n -> Γ.is_rel n := by {
+    generalize HA': expr type A = A';
+    rw [HA'] at H;
+    induction H with
+    | var HA Hv _IA =>
+      intro H;
+      cases H; 
+      cases HA';
+      exists A
+    | _ => cases HA' <;> sorry
+  }
